mem/Open.v
@@ -107,29 +107,6 @@ Section ADQ.
   (* Proof. refl. Qed. *)
 
 
-  Ltac resub :=
-    repeat multimatch goal with
-           | |- context[ITree.trigger ?e] =>
-             match e with
-             | subevent _ _ => idtac
-             | _ => replace (ITree.trigger e) with (trigger e) by refl
-             end
-           | |- context[@subevent _ ?F ?prf _ (?e|)%sum] =>
-             let my_tac := ltac:(fun H => replace (@subevent _ F prf _ (e|)%sum) with (@subevent _ F _ _ e) by H) in
-             match (type of e) with
-             | (_ +' _) _ => my_tac ltac:(destruct e; refl)
-             | _ => my_tac ltac:(refl)
-             end
-           | |- context[@subevent _ ?F ?prf _ (|?e)%sum] =>
-             let my_tac := ltac:(fun H => replace (@subevent _ F prf _ (|e)%sum) with (@subevent _ F _ _ e) by H) in
-             match (type of e) with
-             | (_ +' _) _ => my_tac ltac:(destruct e; refl)
-             | _ => my_tac ltac:(refl)
-             end
-           | |- context[ITree.trigger (@subevent _ ?F ?prf _ (resum ?a ?b ?e))] =>
-             replace (ITree.trigger (@subevent _ F prf _ (resum a b e))) with (ITree.trigger (@subevent _ F _ _ e)) by refl
-           end.
-
   Lemma add_list_fnsems
         mds ske
     :
